partial and total functions (WIP)

src/Theories/Sorts.v
@@ -1,9 +1,16 @@
+From Coq Require Import ssreflect ssrfun ssrbool.
+Set Implicit Arguments.
+Unset Strict Implicit.
+Unset Printing Implicit Defensive.
+
+From Coq Require Import Unicode.Utf8.
 Require Import Coq.Logic.Classical_Prop.
 
-From MatchingLogic Require Import Syntax.
+From MatchingLogic Require Import Syntax Semantics.
 Require Import MatchingLogic.Theories.Definedness.
 
 Import MatchingLogic.Syntax.Notations.
+Import MatchingLogic.Syntax.BoundVarSugar.
 Import MatchingLogic.Semantics.Notations.
 
 Section sorts.
@@ -21,7 +28,7 @@ Section sorts.
 
   Existing Instance imported_definedness.
 
-  Let sym (s : Symbols) : @Pattern sig :=
+  Local Definition sym (s : Symbols) : @Pattern sig :=
     @patt_sym sig (inj s).
   
   Example test_pattern_1 := patt_equal (sym inhabitant) (sym inhabitant).
@@ -34,5 +41,39 @@ Section sorts.
     patt_exists ((patt_in (patt_bound_evar 0) (inhabitant_set sort)) and phi).
 
   (* TODO patt_forall_of_sort and patt_exists_of_sorts are duals - a lemma *)
+
+  (* TODO a lemma about patt_forall_of_sort *)
   
+  Definition patt_total_function(phi from to : Pattern) : Pattern :=
+    patt_forall_of_sort from (patt_exists_of_sort to (patt_equal (patt_app phi b1) b0)).
+
+  Definition patt_partial_function(phi from to : Pattern) : Pattern :=
+    patt_forall_of_sort from (patt_exists_of_sort to (patt_subseteq (patt_app phi b1) b0)).
+
+  Section with_model.
+    Context {M : Model}.
+    Hypothesis M_satisfies_theory : M ⊨ᵀ Definedness.theory.
+
+    Definition Minhabitant_set m := app_ext (sym_interp (inj inhabitant)) (Ensembles.Singleton (Domain M) m).
+
+    (* ϕ is expected to be a sort pattern *)
+    Definition Minterp_inhabitant ϕ ρₑ ρₛ := @pattern_interpretation sig M ρₑ ρₛ (patt_app (sym inhabitant) ϕ).
+
+    (*Search pattern_interpretation patt_forall.*)
+    
+    Lemma interp_total_function f s₁ s₂ ρₑ ρₛ :
+      @pattern_interpretation sig M ρₑ ρₛ (patt_total_function f s₁ s₂) = Full ->
+      ∀ (m₁ : Domain M),
+        Minterp_inhabitant s₁ ρₑ ρₛ m₁ ->                 
+        ∃ (m₂ : Domain M),
+          Minterp_inhabitant s₂ ρₑ ρₛ m₂ ->
+          app_ext (@pattern_interpretation sig M ρₑ ρₛ f) (Ensembles.Singleton (Domain M) m₁)
+          = Ensembles.Singleton (Domain M) m₂.
+    Proof.
+      intros Hfun m₁ H1.
+      unfold patt_total_function in Hfun.
+    Abort.
+
+  End with_model.
+    
 End sorts.
